

Intro to Robotics HW7

Zhuorui YUN

November 2025

1 Problem 1

A robotic arm has two links with $L_1 = 1.2m$, and $L_2 = 0.8m$. The end effector needs to move from point A $[-1.2, 0.9]$ to B $[1.1, 0.8]$. The end effector weights $m_e = 1kg$ and each link weights $m_1 = m_2 = 1kg$ with uniform distributed mass. A robotic arm has two links with $L_1 = 1.2m$, and $L_2 = 0.8m$. The end effector needs to move from point A $[-1.2, 0.9]$ to B $[1.1, 0.8]$. The end effector weights $m_e = 1kg$ and each link weights $m_1 = m_2 = 1kg$ with uniform distributed mass.

Please write down the kinetic energy T and potential energy V of this system. Please derive the equation of motion, i.e., obtain the expression of τ_1 and τ_2 . Please write down the mass matrix M , centrifugal and Coriolis terms V , and gravity terms G .

1.1 Kinetic Energy T

System Parameters (Given)

- Length of Link 1: $l_1 = 1.2m$
- Length of Link 2: $l_2 = 0.8m$
- Joint Angles: θ_1, θ_2

Mass Properties

- End-effector Mass: m_e
- Mass of Each Link: m

Center of Link Mass

- $l_{c1} = \frac{l_1}{2}$
- $l_{c2} = \frac{l_2}{2}$

Moment of Inertia

- $I_1 = \frac{1}{12}ml_1^2$
- $I_2 = \frac{1}{12}ml_2^2$

Total kinetic Energy

- $T = T_{link1,trans} + T_{link1,rot} + T_{link2,trans} + T_{link2,rot} + T_{end,effector}$

Position Vector

$$P_{c1} = \begin{bmatrix} x_{c1} \\ y_{c1} \end{bmatrix} = \begin{bmatrix} \frac{L_1}{2} \cos \theta_1 \\ \frac{L_1}{2} \sin \theta_1 \end{bmatrix}$$

$$P_{c2} = \begin{bmatrix} x_{c2} \\ y_{c2} \end{bmatrix} = \begin{bmatrix} L_1 \cos \theta_1 + \frac{L_2}{2} \cos(\theta_1 + \theta_2) \\ L_1 \sin \theta_1 + \frac{L_2}{2} \sin(\theta_1 + \theta_2) \end{bmatrix}$$

$$P_e = \begin{bmatrix} x_e \\ y_e \end{bmatrix} = \begin{bmatrix} L_1 \cos \theta_1 + L_2 \cos(\theta_1 + \theta_2) \\ L_1 \sin \theta_1 + L_2 \sin(\theta_1 + \theta_2) \end{bmatrix}$$

Velocity of link1

$$\mathbf{v}_{c1} = \begin{bmatrix} -\frac{L_1}{2} \sin \theta_1 \cdot \dot{\theta}_1 \\ \frac{L_1}{2} \cos \theta_1 \cdot \dot{\theta}_1 \end{bmatrix}$$

$$T_1 = \frac{1}{2} m_1 v_{c1}^2 + \frac{1}{2} I_1 \omega_1^2$$

Velocity of link2

$$\mathbf{v}_{c2} = \begin{bmatrix} -L_1 \sin \theta_1 \dot{\theta}_1 - \frac{L_2}{2} \sin(\theta_1 + \theta_2)(\dot{\theta}_1 + \dot{\theta}_2) \\ L_1 \cos \theta_1 \dot{\theta}_1 + \frac{L_2}{2} \cos(\theta_1 + \theta_2)(\dot{\theta}_1 + \dot{\theta}_2) \end{bmatrix}$$

Velocity of End-effector

$$\mathbf{v}_e = \begin{bmatrix} -L_1 \sin \theta_1 \dot{\theta}_1 - L_2 \sin(\theta_1 + \theta_2)(\dot{\theta}_1 + \dot{\theta}_2) \\ L_1 \cos \theta_1 \dot{\theta}_1 + L_2 \cos(\theta_1 + \theta_2)(\dot{\theta}_1 + \dot{\theta}_2) \end{bmatrix}$$

Kinetic for link 1

$$T_1 = T_{1t} + T_{1r} = \frac{1}{2} m_1 v_{c1}^2 + \frac{1}{2} I_1 \dot{\theta}_1^2$$

where $I_1 = \frac{1}{12} m_1 L_1^2$

$$T_1 = \frac{1}{2} m_1 \left(\frac{L_1}{2} \dot{\theta}_1 \right)^2 + \frac{1}{2} \left(\frac{1}{12} m_1 L_1^2 \right) \dot{\theta}_1^2 = \frac{1}{2} m_1 L_1^2 \left(\frac{1}{4} + \frac{1}{12} \right) \dot{\theta}_1^2 = \frac{1}{6} m_1 L_1^2 \dot{\theta}_1^2$$

Kinetic for link 2

$$T_2 = T_{2t} + T_{2r} = \frac{1}{2} m_2 v_{c2}^2 + \frac{1}{2} I_2 (\dot{\theta}_1 + \dot{\theta}_2)^2$$

where $I_2 = \frac{1}{12} m_2 L_2^2$

$$T_2 = \frac{1}{2} m_2 \left[L_1^2 \dot{\theta}_1^2 + \frac{L_2^2}{4} (\dot{\theta}_1 + \dot{\theta}_2)^2 + 2L_1 L_2 \cos \theta_1 (\dot{\theta}_1 + \dot{\theta}_2) \right] + \frac{1}{2} \left(\frac{1}{12} m_2 L_2^2 \right) (\dot{\theta}_1 + \dot{\theta}_2)^2$$

Kinetic Energy of End Effector (T_e)

$$T_e = \frac{1}{2} m_e v_e^2$$

$$T_e = \frac{1}{2} m_e \left[L_1^2 \dot{\theta}_1^2 + L_2^2 (\dot{\theta}_1 + \dot{\theta}_2)^2 + 2L_1 L_2 \cos \theta_2 \dot{\theta}_1 (\dot{\theta}_1 + \dot{\theta}_2) \right]$$

Total Kinetic Energy T The total kinetic energy is $T = T_1 + T_2 + T_e$. We substitute the given values $L_1 = 1.2$, $L_2 = 0.8$, $m_1 = m_2 = m_e = 1$. $L_1^2 = 1.44$, $L_2^2 = 0.64$, $L_1 L_2 = 0.96$. $I_1 = \frac{1}{12}(1)(1.44) = 0.12$, $I_2 = \frac{1}{12}(1)(0.64) \approx 0.0533$.

$$T_1 = \frac{1}{6}(1)(1.44)\dot{\theta}_1^2 = 0.24\dot{\theta}_1^2$$

$$T_2 = \frac{1}{2}(1) \left[(1.6 + 0.96c_2)\dot{\theta}_1^2 + 0.16\dot{\theta}_2^2 + (0.32 + 0.96c_2)\dot{\theta}_1\dot{\theta}_2 \right] + 0.0267(\dot{\theta}_1 + \dot{\theta}_2)^2$$

$$T_e = \frac{1}{2}(1) \left[(2.08 + 1.92c_2)\dot{\theta}_1^2 + 0.64\dot{\theta}_2^2 + (1.28 + 1.92c_2)\dot{\theta}_1\dot{\theta}_2 \right]$$

Total Kinetic Energy T

$$T = \frac{1}{2} (4.2133 + 2.88c_2) \dot{\theta}_1^2 + \frac{1}{2} (0.8533) \dot{\theta}_2^2 + (0.8533 + 1.44c_2) \dot{\theta}_1 \dot{\theta}_2$$

1.2 Potential Energy

$$V = g \left[m_1 \left(\frac{L_1}{2} s_1 \right) + m_2 \left(L_1 s_1 + \frac{L_2}{2} s_{12} \right) + m_e (L_1 s_1 + L_2 s_{12}) \right]$$

where $m_1 = m_2 = m_e = 1kg$, $L_1 = 0.8m$, $L_2 = 1m$

$$V = g [3.0 \sin \theta_1 + 1.2 \sin(\theta_1 + \theta_2)]$$

Lagrangian and Equation of Motion

The Euler-Lagrange equations for the generalized coordinate q_i (where $q_1 = \theta_1$, $q_2 = \theta_2$) under generalized force τ_i are:

$$\frac{d}{dt} \left(\frac{\partial T}{\partial \dot{q}_i} \right) - \frac{\partial T}{\partial q_i} + \frac{\partial V}{\partial q_i} = \tau_i$$

1.3 Mass Matrix \mathbf{M}

we take the partial derivative for total kinetic energy

$$\frac{\partial T}{\partial \dot{q}} = \begin{bmatrix} (4.2133 + 2.88c_2)\dot{\theta}_1 + (0.8533 + 1.44c_2)\dot{\theta}_2 \\ 0.8533\dot{\theta}_2 + (0.8533 + 1.44c_2)\dot{\theta}_1 \end{bmatrix}$$

$$\mathbf{M}(\mathbf{q}) = \begin{bmatrix} M_{11} & M_{12} \\ M_{21} & M_{22} \end{bmatrix}$$

M_{11} is coefficient of $\dot{\theta}_1$:

$$M_{11} = 4.2133 + 2.88 \cos \theta_2$$

M_{22} is the coefficient of $\frac{1}{2}\dot{\theta}_2^2$:

$$M_{22} = 0.8533$$

$M_{12} = M_{21}$:

$$M_{12} = M_{21} = 0.8533 + 1.44 \cos \theta_2$$

so

$$\mathbf{M} = \begin{bmatrix} 4.2133 + 2.88c_2 & 0.8533 + 1.44c_2 \\ 0.8533 + 1.44c_2 & 0.8533 \end{bmatrix}$$

1.4 Coriolis and Centrifugal Terms (Vector $\mathbf{C}\dot{\mathbf{q}}$)

The Euler-Lagrange equations lead to the general form:

$$\mathbf{M}\ddot{\mathbf{q}} + \mathbf{C}\dot{\mathbf{q}} + \mathbf{G} = \boldsymbol{\tau}$$

It concluding $\dot{M}(q)\dot{q}$ and $-\frac{\partial T}{\partial q_i}$

$$\dot{\mathbf{M}} = \begin{bmatrix} -2.88s_2\dot{\theta}_2 & -1.44s_2\dot{\theta}_2 \\ -1.44s_2\dot{\theta}_2 & 0 \end{bmatrix}$$

$$-\frac{\partial T}{\partial q} = \begin{bmatrix} 0 \\ 1.44s_2\dot{\theta}_1^2 + 1.44s_2\dot{\theta}_1\dot{\theta}_2 \end{bmatrix}$$

$$\dot{M}\dot{q} - \frac{\partial T}{\partial q_i} = \mathbf{C}\dot{\mathbf{q}} = \begin{bmatrix} -2.88s_2\dot{\theta}_1\dot{\theta}_2 - 1.44s_2\dot{\theta}_2^2 \\ -1.44s_2\dot{\theta}_1^2 \end{bmatrix}$$

1.5 Gravity Terms \mathbf{G}

The gravity vector \mathbf{G} is obtained by $\mathbf{G} = \frac{\partial V}{\partial \mathbf{q}}$.

$$\mathbf{G} = \frac{\partial V}{\partial \mathbf{q}} = \begin{bmatrix} g[3\cos\theta_1 + 1.2\cos(\theta_1 + \theta_2)] \\ g1.2\cos(\theta_1 + \theta_2) \end{bmatrix}$$

1.6 Torques($\boldsymbol{\tau}$)

The required torques $\boldsymbol{\tau} = [\tau_1, \tau_2]^T$ are given by the equation :

$$\begin{bmatrix} \tau_1 \\ \tau_2 \end{bmatrix} = \mathbf{M}(\mathbf{q})\ddot{\mathbf{q}} + \mathbf{C}(\mathbf{q}, \dot{\mathbf{q}}) + \mathbf{G}(\mathbf{q})$$

$$\tau_1 = (4.2133 + 2.88c_2)\ddot{\theta}_1 + (0.8533 + 1.44c_2)\ddot{\theta}_2 - 2.88s_2\dot{\theta}_1\dot{\theta}_2 - 1.44s_2\dot{\theta}_2^2 + g[3c_1 + 1.2c_{12}]$$

$$\tau_2 = (0.8533 + 1.44c_2)\ddot{\theta}_1 + 0.8533\ddot{\theta}_2 - 1.44s_2\dot{\theta}_1^2 + g1.2c_{12}$$